examples/pseudo_bool/cp_encoding/cp_to_ilp_arrayScript.sml
@@ -1,0 +1,156 @@
+(*
+  Formalization of the CP to ILP phase (array constraints)
+*)
+Theory cp_to_ilp_array
+Libs
+  preamble
+Ancestors
+  pbc cp ilp cp_to_ilp
+
+(* Element: Xs[Y - offset] = Z *)
+Definition encode_element_def:
+  encode_element bnd Xs Yi Z =
+  [false_constr]
+End
+
+Theorem encode_element_sem_1:
+  valid_assignment bnd wi ∧
+  element_sem Xs Yi Z wi ⇒
+  EVERY (λx. iconstraint_sem x (wi,reify_avar cs wi))
+    (encode_element bnd Xs Yi Z)
+Proof
+  cheat
+QED
+
+Theorem encode_element_sem_2:
+  valid_assignment bnd wi ∧
+  EVERY (λx. iconstraint_sem x (wi,wb))
+    (encode_element bnd Xs Yi Z) ⇒
+  element_sem Xs Yi Z wi
+Proof
+  cheat
+QED
+
+(* Element2D: Xss[Y1 - offset1][Y2 - offset2] = Z *)
+Definition encode_element2d_def:
+  encode_element2d bnd Xss Y1i Y2i Z =
+  [false_constr]
+End
+
+Theorem encode_element2d_sem_1:
+  valid_assignment bnd wi ∧
+  element2d_sem Xss Y1i Y2i Z wi ⇒
+  EVERY (λx. iconstraint_sem x (wi,reify_avar cs wi))
+    (encode_element2d bnd Xss Y1i Y2i Z)
+Proof
+  cheat
+QED
+
+Theorem encode_element2d_sem_2:
+  valid_assignment bnd wi ∧
+  EVERY (λx. iconstraint_sem x (wi,wb))
+    (encode_element2d bnd Xss Y1i Y2i Z) ⇒
+  element2d_sem Xss Y1i Y2i Z wi
+Proof
+  cheat
+QED
+
+(* ArrayMax: Y = max(Xs) *)
+Definition encode_array_max_def:
+  encode_array_max bnd Xs Y =
+  [false_constr]
+End
+
+Theorem encode_array_max_sem_1:
+  valid_assignment bnd wi ∧
+  array_max_sem Xs Y wi ⇒
+  EVERY (λx. iconstraint_sem x (wi,reify_avar cs wi))
+    (encode_array_max bnd Xs Y)
+Proof
+  cheat
+QED
+
+Theorem encode_array_max_sem_2:
+  valid_assignment bnd wi ∧
+  EVERY (λx. iconstraint_sem x (wi,wb))
+    (encode_array_max bnd Xs Y) ⇒
+  array_max_sem Xs Y wi
+Proof
+  cheat
+QED
+
+(* ArrayMin: Y = min(Xs) *)
+Definition encode_array_min_def:
+  encode_array_min bnd Xs Y =
+  [false_constr]
+End
+
+Theorem encode_array_min_sem_1:
+  valid_assignment bnd wi ∧
+  array_min_sem Xs Y wi ⇒
+  EVERY (λx. iconstraint_sem x (wi,reify_avar cs wi))
+    (encode_array_min bnd Xs Y)
+Proof
+  cheat
+QED
+
+Theorem encode_array_min_sem_2:
+  valid_assignment bnd wi ∧
+  EVERY (λx. iconstraint_sem x (wi,wb))
+    (encode_array_min bnd Xs Y) ⇒
+  array_min_sem Xs Y wi
+Proof
+  cheat
+QED
+
+Definition encode_array_constr_def:
+  encode_array_constr bnd c name =
+  case c of
+    Element Xs Yi Z => encode_element bnd Xs Yi Z
+  | Element2D Xss Y1i Y2i Z => encode_element2d bnd Xss Y1i Y2i Z
+  | ArrayMax Xs Y => encode_array_max bnd Xs Y
+  | ArrayMin Xs Y => encode_array_min bnd Xs Y
+End
+
+Theorem encode_array_constr_sem_1:
+  valid_assignment bnd wi ∧
+  ALOOKUP cs name = SOME (Array c) ∧
+  array_constr_sem c wi ⇒
+  EVERY (λx. iconstraint_sem x (wi,reify_avar cs wi))
+    (encode_array_constr bnd c name)
+Proof
+  Cases_on`c`>>
+  rw[encode_array_constr_def,array_constr_sem_def]
+  >- metis_tac[encode_element_sem_1]
+  >- metis_tac[encode_element2d_sem_1]
+  >- metis_tac[encode_array_max_sem_1]
+  >- metis_tac[encode_array_min_sem_1]
+QED
+
+Theorem encode_array_constr_sem_2:
+  valid_assignment bnd wi ∧
+  EVERY (λx. iconstraint_sem x (wi,wb))
+    (encode_array_constr bnd c name) ⇒
+  array_constr_sem c wi
+Proof
+  Cases_on`c`>>
+  rw[encode_array_constr_def,array_constr_sem_def]
+  >- metis_tac[encode_element_sem_2]
+  >- metis_tac[encode_element2d_sem_2]
+  >- metis_tac[encode_array_max_sem_2]
+  >- metis_tac[encode_array_min_sem_2]
+QED
+
+(* Concrete encodings *)
+Definition cencode_array_constr_def:
+  cencode_array_constr bnd c name ec =
+  (List [], ec)
+End
+
+Theorem cencode_array_constr_sem:
+  valid_assignment bnd wi ∧
+  cencode_array_constr bnd c name ec = (es, ec') ⇒
+  enc_rel wi es (encode_array_constr bnd c name) ec ec'
+Proof
+  cheat
+QED
