examples/pseudo_bool/cp_encoding/cp_to_ilp_channelingScript.sml
@@ -1,0 +1,91 @@
+(*
+  Formalization of the CP to ILP phase (channeling constraints)
+*)
+Theory cp_to_ilp_channeling
+Libs
+  preamble
+Ancestors
+  pbc cp ilp cp_to_ilp
+
+(* Inverse: Xs and Ys are inverse permutations
+   Xs[i] = j ⇔ Ys[j] = i
+   This is very complex as it involves bidirectional constraints
+*)
+Definition encode_inverse_def:
+  encode_inverse bnd Xsi Ysi =
+  let (Xs,offx) = Xsi in
+  let (Ys,offy) = Ysi in
+  let n = LENGTH Xs in
+  if n ≠ LENGTH Ys then
+    [false_constr]
+  else
+    (* Bounds constraints *)
+    MAP (λX. mk_constraint_ge 1 X (-1) (INR offy) 0) Xs ++
+    MAP (λX. mk_constraint_ge (-1) X (1) (INR (offy + &n)) (-1)) Xs ++
+    MAP (λY. mk_constraint_ge 1 Y (-1) (INR offx) 0) Ys ++
+    MAP (λY. mk_constraint_ge (-1) Y (1) (INR (offx + &n)) (-1)) Ys ++
+    (* Channeling constraints: Xs[i] = j ⇔ Ys[j] = i
+       This requires complex encoding with element constraints *)
+    [false_constr]
+End
+
+Theorem encode_inverse_sem_1:
+  valid_assignment bnd wi ∧
+  inverse_sem Xsi Ysi wi ⇒
+  EVERY (λx. iconstraint_sem x (wi,reify_avar cs wi))
+    (encode_inverse bnd Xsi Ysi)
+Proof
+  cheat
+QED
+
+Theorem encode_inverse_sem_2:
+  valid_assignment bnd wi ∧
+  EVERY (λx. iconstraint_sem x (wi,wb))
+    (encode_inverse bnd Xsi Ysi) ⇒
+  inverse_sem Xsi Ysi wi
+Proof
+  cheat
+QED
+
+Definition encode_channeling_constr_def:
+  encode_channeling_constr bnd c name =
+  case c of Inverse Xsi Ysi =>
+    encode_inverse bnd Xsi Ysi
+End
+
+Theorem encode_channeling_constr_sem_1:
+  valid_assignment bnd wi ∧
+  ALOOKUP cs name = SOME (Channeling c) ∧
+  channeling_constr_sem c wi ⇒
+  EVERY (λx. iconstraint_sem x (wi,reify_avar cs wi))
+    (encode_channeling_constr bnd c name)
+Proof
+  Cases_on`c`>>
+  rw[encode_channeling_constr_def,channeling_constr_sem_def]>>
+  metis_tac[encode_inverse_sem_1]
+QED
+
+Theorem encode_channeling_constr_sem_2:
+  valid_assignment bnd wi ∧
+  EVERY (λx. iconstraint_sem x (wi,wb))
+    (encode_channeling_constr bnd c name) ⇒
+  channeling_constr_sem c wi
+Proof
+  Cases_on`c`>>
+  rw[encode_channeling_constr_def,channeling_constr_sem_def]>>
+  metis_tac[encode_inverse_sem_2]
+QED
+
+(* Concrete encodings - TODO *)
+Definition cencode_channeling_constr_def:
+  cencode_channeling_constr bnd c name ec =
+  (List [], ec)
+End
+
+Theorem cencode_channeling_constr_sem:
+  valid_assignment bnd wi ∧
+  cencode_channeling_constr bnd c name ec = (es, ec') ⇒
+  enc_rel wi es (encode_channeling_constr bnd c name) ec ec'
+Proof
+  cheat
+QED
