examples/pseudo_bool/cp_encoding/cp_to_ilp_countingScript.sml
@@ -1,0 +1,172 @@
+(*
+  Formalization of the CP to ILP phase (counting constraints)
+*)
+Theory cp_to_ilp_counting
+Libs
+  preamble
+Ancestors
+  pbc cp ilp cp_to_ilp
+
+(* AllDifferent: All variables must take distinct values
+   For n variables, this requires O(n^2) pairwise inequality constraints *)
+Definition encode_all_different_def:
+  encode_all_different bnd Xs =
+  FLAT (MAPi (λi X.
+    FLAT (MAPi (λj Y.
+      if i < j then
+        (* X ≠ Y encoded as (X - Y ≥ 1) ∨ (Y - X ≥ 1) *)
+        (* This requires reification *)
+        [false_constr]
+      else []) Xs)) Xs)
+End
+
+Theorem encode_all_different_sem_1:
+  valid_assignment bnd wi ∧
+  all_different_sem Xs wi ⇒
+  EVERY (λx. iconstraint_sem x (wi,reify_avar cs wi))
+    (encode_all_different bnd Xs)
+Proof
+  cheat
+QED
+
+Theorem encode_all_different_sem_2:
+  valid_assignment bnd wi ∧
+  EVERY (λx. iconstraint_sem x (wi,wb))
+    (encode_all_different bnd Xs) ⇒
+  all_different_sem Xs wi
+Proof
+  cheat
+QED
+
+(* NValue: Y equals the number of distinct values in Xs
+   This is very complex and requires auxiliary variables *)
+Definition encode_n_value_def:
+  encode_n_value bnd Xs Y =
+  (* TODO: Complex encoding requiring auxiliary variables
+     for each potential value in the domain *)
+  [false_constr]
+End
+
+Theorem encode_n_value_sem_1:
+  valid_assignment bnd wi ∧
+  n_value_sem Xs Y wi ⇒
+  EVERY (λx. iconstraint_sem x (wi,reify_avar cs wi))
+    (encode_n_value bnd Xs Y)
+Proof
+  cheat
+QED
+
+Theorem encode_n_value_sem_2:
+  valid_assignment bnd wi ∧
+  EVERY (λx. iconstraint_sem x (wi,wb))
+    (encode_n_value bnd Xs Y) ⇒
+  n_value_sem Xs Y wi
+Proof
+  cheat
+QED
+
+(* Count: Z equals the number of times Y appears in Xs
+   Z = Sum_i [Xs[i] = Y] *)
+Definition encode_count_def:
+  encode_count bnd Xs Y Z =
+  (* Need to encode: Z = Sum_i (Xs[i] = Y)
+     This requires equality reification for each Xs[i] = Y *)
+  [false_constr]
+End
+
+Theorem encode_count_sem_1:
+  valid_assignment bnd wi ∧
+  count_sem Xs Y Z wi ⇒
+  EVERY (λx. iconstraint_sem x (wi,reify_avar cs wi))
+    (encode_count bnd Xs Y Z)
+Proof
+  cheat
+QED
+
+Theorem encode_count_sem_2:
+  valid_assignment bnd wi ∧
+  EVERY (λx. iconstraint_sem x (wi,wb))
+    (encode_count bnd Xs Y Z) ⇒
+  count_sem Xs Y Z wi
+Proof
+  cheat
+QED
+
+(* Among: Y equals the number of times values from iS appear in Xs
+   Y = Sum_i [Xs[i] ∈ iS] *)
+Definition encode_among_def:
+  encode_among bnd Xs iS Y =
+  (* Need to encode: Y = Sum_i (Xs[i] ∈ iS)
+     For each i, need disjunction: Xs[i] = v1 ∨ Xs[i] = v2 ∨ ... *)
+  [false_constr]
+End
+
+Theorem encode_among_sem_1:
+  valid_assignment bnd wi ∧
+  among_sem Xs iS Y wi ⇒
+  EVERY (λx. iconstraint_sem x (wi,reify_avar cs wi))
+    (encode_among bnd Xs iS Y)
+Proof
+  cheat
+QED
+
+Theorem encode_among_sem_2:
+  valid_assignment bnd wi ∧
+  EVERY (λx. iconstraint_sem x (wi,wb))
+    (encode_among bnd Xs iS Y) ⇒
+  among_sem Xs iS Y wi
+Proof
+  cheat
+QED
+
+Definition encode_counting_constr_def:
+  encode_counting_constr bnd c name =
+  case c of
+    AllDifferent Xs => encode_all_different bnd Xs
+  | NValue Xs Y => encode_n_value bnd Xs Y
+  | Count Xs Y Z => encode_count bnd Xs Y Z
+  | Among Xs iS Y => encode_among bnd Xs iS Y
+End
+
+Theorem encode_counting_constr_sem_1:
+  valid_assignment bnd wi ∧
+  ALOOKUP cs name = SOME (Counting c) ∧
+  counting_constr_sem c wi ⇒
+  EVERY (λx. iconstraint_sem x (wi,reify_avar cs wi))
+    (encode_counting_constr bnd c name)
+Proof
+  Cases_on`c`>>
+  rw[encode_counting_constr_def,counting_constr_sem_def]
+  >- metis_tac[encode_all_different_sem_1]
+  >- metis_tac[encode_n_value_sem_1]
+  >- metis_tac[encode_count_sem_1]
+  >- metis_tac[encode_among_sem_1]
+QED
+
+Theorem encode_counting_constr_sem_2:
+  valid_assignment bnd wi ∧
+  EVERY (λx. iconstraint_sem x (wi,wb))
+    (encode_counting_constr bnd c name) ⇒
+  counting_constr_sem c wi
+Proof
+  Cases_on`c`>>
+  rw[encode_counting_constr_def,counting_constr_sem_def]
+  >- metis_tac[encode_all_different_sem_2]
+  >- metis_tac[encode_n_value_sem_2]
+  >- metis_tac[encode_count_sem_2]
+  >- metis_tac[encode_among_sem_2]
+QED
+
+(* Concrete encodings - TODO *)
+Definition cencode_counting_constr_def:
+  cencode_counting_constr bnd c name ec =
+  (List [], ec)
+End
+
+Theorem cencode_counting_constr_sem:
+  valid_assignment bnd wi ∧
+  cencode_counting_constr bnd c name ec = (es, ec') ⇒
+  enc_rel wi es (encode_counting_constr bnd c name) ec ec'
+Proof
+  cheat
+QED
