examples/pseudo_bool/cp_encoding/cp_to_ilp_lexicographicalScript.sml
@@ -1,0 +1,87 @@
+(*
+  Formalization of the CP to ILP phase (lexicographical constraints)
+*)
+Theory cp_to_ilp_lexicographical
+Libs
+  preamble
+Ancestors
+  pbc cp ilp cp_to_ilp
+
+(* Lexicographical comparison: Xs lex_cmp Ys
+   For Xs < Ys lexicographically:
+   ∃i. (∀j < i. Xs[j] = Ys[j]) ∧ Xs[i] < Ys[i]
+
+   This requires auxiliary variables to track the position of first difference
+*)
+Definition encode_lex_def:
+  encode_lex bnd cmp Xs Ys =
+  if LENGTH Xs ≠ LENGTH Ys then
+    [false_constr]
+  else
+    (* Complex encoding requiring auxiliary variables for:
+       1. Position of first difference
+       2. All elements before that position are equal
+       3. Comparison at that position *)
+    [false_constr]
+End
+
+Theorem encode_lex_sem_1:
+  valid_assignment bnd wi ∧
+  lex_sem cmp Xs Ys wi ⇒
+  EVERY (λx. iconstraint_sem x (wi,reify_avar cs wi))
+    (encode_lex bnd cmp Xs Ys)
+Proof
+  cheat
+QED
+
+Theorem encode_lex_sem_2:
+  valid_assignment bnd wi ∧
+  EVERY (λx. iconstraint_sem x (wi,wb))
+    (encode_lex bnd cmp Xs Ys) ⇒
+  lex_sem cmp Xs Ys wi
+Proof
+  cheat
+QED
+
+Definition encode_lexicographical_constr_def:
+  encode_lexicographical_constr bnd c name =
+  case c of Lex cmp Xs Ys =>
+    encode_lex bnd cmp Xs Ys
+End
+
+Theorem encode_lexicographical_constr_sem_1:
+  valid_assignment bnd wi ∧
+  ALOOKUP cs name = SOME (Lexicographical c) ∧
+  lexicographical_constr_sem c wi ⇒
+  EVERY (λx. iconstraint_sem x (wi,reify_avar cs wi))
+    (encode_lexicographical_constr bnd c name)
+Proof
+  Cases_on`c`>>
+  rw[encode_lexicographical_constr_def,lexicographical_constr_sem_def]>>
+  metis_tac[encode_lex_sem_1]
+QED
+
+Theorem encode_lexicographical_constr_sem_2:
+  valid_assignment bnd wi ∧
+  EVERY (λx. iconstraint_sem x (wi,wb))
+    (encode_lexicographical_constr bnd c name) ⇒
+  lexicographical_constr_sem c wi
+Proof
+  Cases_on`c`>>
+  rw[encode_lexicographical_constr_def,lexicographical_constr_sem_def]>>
+  metis_tac[encode_lex_sem_2]
+QED
+
+(* Concrete encodings - TODO *)
+Definition cencode_lexicographical_constr_def:
+  cencode_lexicographical_constr bnd c name ec =
+  (List [], ec)
+End
+
+Theorem cencode_lexicographical_constr_sem:
+  valid_assignment bnd wi ∧
+  cencode_lexicographical_constr bnd c name ec = (es, ec') ⇒
+  enc_rel wi es (encode_lexicographical_constr bnd c name) ec ec'
+Proof
+  cheat
+QED
