examples/pseudo_bool/cp_encoding/cp_to_ilp_linearScript.sml
@@ -1,0 +1,76 @@
+(*
+  Formalization of the CP to ILP phase (linear constraints)
+*)
+Theory cp_to_ilp_linear
+Libs
+  preamble
+Ancestors
+  pbc cp ilp cp_to_ilp
+
+(* Linear constraint: Σ ci·Xi cmp Y *)
+Definition encode_lin_def:
+  encode_lin bnd Zr cmp Xs Y =
+  [false_constr]
+End
+
+Theorem encode_lin_sem_1:
+  valid_assignment bnd wi ∧
+  ALOOKUP cs name = SOME (Linear (Lin Zr cmp Xs Y)) ∧
+  lin_sem Zr cmp Xs Y wi ⇒
+  EVERY (λx. iconstraint_sem x (wi,reify_avar cs wi))
+    (encode_lin bnd Zr cmp Xs Y)
+Proof
+  cheat
+QED
+
+Theorem encode_lin_sem_2:
+  valid_assignment bnd wi ∧
+  EVERY (λx. iconstraint_sem x (wi,wb))
+    (encode_lin bnd Zr cmp Xs Y) ⇒
+  lin_sem Zr cmp Xs Y wi
+Proof
+  cheat
+QED
+
+Definition encode_linear_constr_def:
+  encode_linear_constr bnd c name =
+  case c of Lin Zr cmp Xs Y =>
+    encode_lin bnd Zr cmp Xs Y
+End
+
+Theorem encode_linear_constr_sem_1:
+  valid_assignment bnd wi ∧
+  ALOOKUP cs name = SOME (Linear c) ∧
+  linear_constr_sem c wi ⇒
+  EVERY (λx. iconstraint_sem x (wi,reify_avar cs wi))
+    (encode_linear_constr bnd c name)
+Proof
+  Cases_on`c`>>
+  rw[encode_linear_constr_def,linear_constr_sem_def]>>
+  metis_tac[encode_lin_sem_1]
+QED
+
+Theorem encode_linear_constr_sem_2:
+  valid_assignment bnd wi ∧
+  EVERY (λx. iconstraint_sem x (wi,wb))
+    (encode_linear_constr bnd c name) ⇒
+  linear_constr_sem c wi
+Proof
+  Cases_on`c`>>
+  rw[encode_linear_constr_def,linear_constr_sem_def]>>
+  metis_tac[encode_lin_sem_2]
+QED
+
+(* Concrete encodings *)
+Definition cencode_linear_constr_def:
+  cencode_linear_constr bnd c name ec =
+  (List [], ec)
+End
+
+Theorem cencode_linear_constr_sem:
+  valid_assignment bnd wi ∧
+  cencode_linear_constr bnd c name ec = (es, ec') ⇒
+  enc_rel wi es (encode_linear_constr bnd c name) ec ec'
+Proof
+  cheat
+QED
