examples/pseudo_bool/cp_encoding/cp_to_ilp_logicalScript.sml
@@ -1,0 +1,129 @@
+(*
+  Formalization of the CP to ILP phase (logical constraints)
+*)
+Theory cp_to_ilp_logical
+Libs
+  preamble
+Ancestors
+  pbc cp ilp cp_to_ilp
+
+(* And constraint: Y > 0 ⇔ ∀i. Xs[i] > 0 *)
+Definition encode_and_def:
+  encode_and bnd Xs Y =
+  [false_constr]
+End
+
+Theorem encode_and_sem_1:
+  valid_assignment bnd wi ∧
+  and_sem Xs Y wi ⇒
+  EVERY (λx. iconstraint_sem x (wi,reify_avar cs wi))
+    (encode_and bnd Xs Y)
+Proof
+  cheat
+QED
+
+Theorem encode_and_sem_2:
+  valid_assignment bnd wi ∧
+  EVERY (λx. iconstraint_sem x (wi,wb))
+    (encode_and bnd Xs Y) ⇒
+  and_sem Xs Y wi
+Proof
+  cheat
+QED
+
+(* Or constraint: Y > 0 ⇔ ∃i. Xs[i] > 0 *)
+Definition encode_or_def:
+  encode_or bnd Xs Y =
+  [false_constr]
+End
+
+Theorem encode_or_sem_1:
+  valid_assignment bnd wi ∧
+  or_sem Xs Y wi ⇒
+  EVERY (λx. iconstraint_sem x (wi,reify_avar cs wi))
+    (encode_or bnd Xs Y)
+Proof
+  cheat
+QED
+
+Theorem encode_or_sem_2:
+  valid_assignment bnd wi ∧
+  EVERY (λx. iconstraint_sem x (wi,wb))
+    (encode_or bnd Xs Y) ⇒
+  or_sem Xs Y wi
+Proof
+  cheat
+QED
+
+(* Parity constraint: ODD number of Xs[i] > 0 *)
+Definition encode_parity_def:
+  encode_parity bnd Xs =
+  [false_constr]
+End
+
+Theorem encode_parity_sem_1:
+  valid_assignment bnd wi ∧
+  parity_sem Xs wi ⇒
+  EVERY (λx. iconstraint_sem x (wi,reify_avar cs wi))
+    (encode_parity bnd Xs)
+Proof
+  cheat
+QED
+
+Theorem encode_parity_sem_2:
+  valid_assignment bnd wi ∧
+  EVERY (λx. iconstraint_sem x (wi,wb))
+    (encode_parity bnd Xs) ⇒
+  parity_sem Xs wi
+Proof
+  cheat
+QED
+
+Definition encode_logical_constr_def:
+  encode_logical_constr bnd c name =
+  case c of
+    And Xs Y => encode_and bnd Xs Y
+  | Or Xs Y => encode_or bnd Xs Y
+  | Parity Xs => encode_parity bnd Xs
+End
+
+Theorem encode_logical_constr_sem_1:
+  valid_assignment bnd wi ∧
+  ALOOKUP cs name = SOME (Logical c) ∧
+  logical_constr_sem c wi ⇒
+  EVERY (λx. iconstraint_sem x (wi,reify_avar cs wi))
+    (encode_logical_constr bnd c name)
+Proof
+  Cases_on`c`>>
+  rw[encode_logical_constr_def,logical_constr_sem_def]
+  >- metis_tac[encode_and_sem_1]
+  >- metis_tac[encode_or_sem_1]
+  >- metis_tac[encode_parity_sem_1]
+QED
+
+Theorem encode_logical_constr_sem_2:
+  valid_assignment bnd wi ∧
+  EVERY (λx. iconstraint_sem x (wi,wb))
+    (encode_logical_constr bnd c name) ⇒
+  logical_constr_sem c wi
+Proof
+  Cases_on`c`>>
+  rw[encode_logical_constr_def,logical_constr_sem_def]
+  >- metis_tac[encode_and_sem_2]
+  >- metis_tac[encode_or_sem_2]
+  >- metis_tac[encode_parity_sem_2]
+QED
+
+(* Concrete encodings *)
+Definition cencode_logical_constr_def:
+  cencode_logical_constr bnd c name ec =
+  (List [], ec)
+End
+
+Theorem cencode_logical_constr_sem:
+  valid_assignment bnd wi ∧
+  cencode_logical_constr bnd c name ec = (es, ec') ⇒
+  enc_rel wi es (encode_logical_constr bnd c name) ec ec'
+Proof
+  cheat
+QED
