examples/pseudo_bool/cp_encoding/cp_to_ilp_miscScript.sml
@@ -1,0 +1,51 @@
+(*
+  Formalization of the CP to ILP phase (misc constraints)
+*)
+Theory cp_to_ilp_misc
+Libs
+  preamble
+Ancestors
+  pbc cp ilp cp_to_ilp
+
+(* Misc constraints are not yet implemented in the CP semantics
+   (misc_constr_sem always returns T)
+   These are placeholders for future work *)
+
+Definition encode_misc_constr_def:
+  encode_misc_constr bnd c name =
+  []
+End
+
+Theorem encode_misc_constr_sem_1:
+  valid_assignment bnd wi ∧
+  ALOOKUP cs name = SOME (Misc c) ∧
+  misc_constr_sem c wi ⇒
+  EVERY (λx. iconstraint_sem x (wi,reify_avar cs wi))
+    (encode_misc_constr bnd c name)
+Proof
+  rw[encode_misc_constr_def]
+QED
+
+Theorem encode_misc_constr_sem_2:
+  valid_assignment bnd wi ∧
+  EVERY (λx. iconstraint_sem x (wi,wb))
+    (encode_misc_constr bnd c name) ⇒
+  misc_constr_sem c wi
+Proof
+  rw[encode_misc_constr_def,misc_constr_sem_def]
+QED
+
+(* Concrete encodings *)
+Definition cencode_misc_constr_def:
+  cencode_misc_constr bnd c name ec =
+  (List [], ec)
+End
+
+Theorem cencode_misc_constr_sem:
+  valid_assignment bnd wi ∧
+  cencode_misc_constr bnd c name ec = (es, ec') ⇒
+  enc_rel wi es (encode_misc_constr bnd c name) ec ec'
+Proof
+  rw[cencode_misc_constr_def,encode_misc_constr_def]>>
+  simp[enc_rel_def]
+QED
