examples/pseudo_bool/cp_encoding/README.md
@@ -15,8 +15,29 @@ Formalization of the CP to ILP phase (shared infrastructure)
 [cp_to_ilp_allScript.sml](cp_to_ilp_allScript.sml):
 Formalization of the CP to ILP phase (all together)
 
+[cp_to_ilp_arrayScript.sml](cp_to_ilp_arrayScript.sml):
+Formalization of the CP to ILP phase (array constraints)
+
+[cp_to_ilp_channelingScript.sml](cp_to_ilp_channelingScript.sml):
+Formalization of the CP to ILP phase (channeling constraints)
+
+[cp_to_ilp_countingScript.sml](cp_to_ilp_countingScript.sml):
+Formalization of the CP to ILP phase (counting constraints)
+
 [cp_to_ilp_extensionalScript.sml](cp_to_ilp_extensionalScript.sml):
 Formalization of the CP to ILP phase (extensional constraints)
+
+[cp_to_ilp_lexicographicalScript.sml](cp_to_ilp_lexicographicalScript.sml):
+Formalization of the CP to ILP phase (lexicographical constraints)
+
+[cp_to_ilp_linearScript.sml](cp_to_ilp_linearScript.sml):
+Formalization of the CP to ILP phase (linear constraints)
+
+[cp_to_ilp_logicalScript.sml](cp_to_ilp_logicalScript.sml):
+Formalization of the CP to ILP phase (logical constraints)
+
+[cp_to_ilp_miscScript.sml](cp_to_ilp_miscScript.sml):
+Formalization of the CP to ILP phase (misc constraints)
 
 [cp_to_ilp_primScript.sml](cp_to_ilp_primScript.sml):
 Formalization of the CP to ILP phase (prim constraints)
